Working hoare validator

theories/hoare.v
@@ -13,64 +13,19 @@ Set Implicit Arguments.
 Unset Strict Implicit.
 Unset Printing Implicit Defensive.
 
-(** To reason about impure computations, we introduce the “Hoare
-    monad,” also called the “specification monad.” An instance of the
-    specification monad is a couple of [pre] and [post] conditions,
-    such that [pre p T] means the program specified by [p] can be
-    executed safely from a state [T], and [post p T x T'] means the
-    execution of [p] from [T] may compute a result [x] and bring the
-    system to a state [T'].
-
-    We equip this couple of predicate with a [bind] function to
-    sequentially compose specifications. *)
+(** Pre/post specifications and abstract Hoare validity. *)
 
 Local Open Scope classical_set_scope.
 Local Open Scope monae_scope.
-(* model *)
-Module Hoare.
-(* Section tmp. *)
-
-(* Context {T : UU0} {M : stateMonad T} {U : UU0}. *)
-
-(* Variable triple :
-  forall U : UU0, *)
-
-(* Definition Pre := set T. *)
-(* Definition Post (U : UU0) := T -> U -> set T. *)
-(* Program Definition HoareState (pre : Pre) {U : UU0} (post : Post U) : UU0 *)
-(* := *)
-  (* {m : M U | *)
-    (* forall initial, pre initial -> *)
-      (* triple (fun s => s = initial) m (post initial)}. *)
-
-(* Definition top := fun x:T => True. *)
-
-(* Program Definition re (U : UU0) *)
-(* : forall x , @HoareState top U (fun i y f => i = f /\ y = x ) := _. *)
-(* Next Obligation. move=>A a /=. apply: (proj1_sig). apply: Ret. Qed. *)
-
-(* Check HoareState. *)
-(* End tmp. *)
-
-
 
 Record hoare T U : Type := mk_hoare {
   pre : set T ;
-  (* prog : M U  ; *)
   post : T -> U -> set T }.
-(* End tmph. *)
+Arguments mk_hoare {T U} (pre post).
+Arguments pre {T U} (_ _).
+Arguments post {T U} (_ _ _).
 
-
-
-Arguments mk_hoare {T  U} (pre post).
-Arguments pre {T  U} (_ _).
-(* Arguments prog {T M U} _. *)
-Arguments post {T  U} (_ _ _).
-HB.about stateRunMonad.
-
-
-(* Section tmp.  *)
-(* Context T U {M : stateMonad T} (triple : set T -> M U -> (U -> set T) -> Prop). *)
+Module Hoare.
 Definition hoare_ret {T} {U : UU0} (x : U) : @hoare T U :=
   mk_hoare [set: T] (fun s y s' => (x = y) /\ (s = s')).
 
@@ -79,47 +34,8 @@ Definition hoare_bind {T} {U V}
     (fun s => pre m s /\ (forall x, post m s x `<=` pre (k x)))
     (fun s x s2 => exists y s', post m s y s' /\ post (k y) s' x s2).
 
-Inductive valid_hoare {T : UU0} {N : monad} {M: stateRunMonad T N} {U : UU0}
-    (h : hoare T U) (m : M U) : Prop :=
-| correct_hoare : (forall s, pre h s ->
-  (forall a s', (runStateT m s = Ret (a, s')) -> post h s a s')) ->
-  valid_hoare h m.
-
-Notation "{{ pre }} prog {{ post }}" := (valid_hoare (@mk_hoare _ _ pre post) prog)
-  (at level 90,
-   format "'[' '[' {{  pre  }}  ']' '/ ' '['  prog ']' '['  {{  post  }} ']' ']'")
-.
-Check correct_hoare.
-Check forall x, pre (hoare_ret x).
-
-Section tmp.
-Hypothesis injective_return : forall (M : monad) (C : Type) (x1 x2 : C),
-  Ret x1 = (Ret x2 :> M C) -> x1 = x2.
-
-Lemma valid_ret {T: UU0} {U : UU0} {N : monad} {M : stateRunMonad T N} (x : U)
-  : @valid_hoare T N M U (@hoare_ret T U x) (Ret x).
-apply: correct_hoare => //=.
-move=> s P u s'.
-HB.about stateRunMonad.
-rewrite runStateTret /==> Hret.
-by have [] := @injective_return N (U * T) (x,s) (u,s') Hret.
-Qed.
-
-Lemma valid_bind {T: UU0} {U V : UU0} {N : monad} {M : stateRunMonad T N}
-  (h : hoare T U) ( m : M U) (h' : U -> hoare T V) (k : U -> M V)
-  : @valid_hoare T N M V (hoare_bind h h' ) (m >>= k).
-Proof.
-apply: correct_hoare=> //=.
-move=> s [Hpr Hpo] v s'.
-rewrite runStateTbind /=.
-(* case: (runStateT m s). *)
-(* exists . *)
-Admitted.
-End tmp.
-
 Section hm.
 Context (T : UU0).
- (* {M : stateMonad T}. *)
 Let ret := @hoare_ret T.
 Let bind := @hoare_bind T.
 
@@ -128,13 +44,10 @@ Proof.
 move=> A [pr po].
 rewrite /bind /ret /hoare_bind /hoare_ret/=; congr mk_hoare.
 - by apply/seteqP; split => // s [].
-(* - exact: bindmret. *)
 - apply/eq3_fun => s a s''.
   under eq2_exists do rewrite andA.
   by rewrite ex2C ex2_eqr ex_eqr.
 Qed.
-
-(* Local Open Scope ssripat_scope. *)
 
 Let left_neutral : BindLaws.left_neutral bind ret.
 Proof.
@@ -143,7 +56,6 @@ move fa : (f a) => [pr po]; congr mk_hoare.
 - apply/funext=> s; rewrite andTP; apply/propext; split.
   + by move=> /(_ a s); rewrite fa/=; exact.
   + by move=> prs _ _ [<- <-]; rewrite fa.
-(* - by rewrite bindretf fa. *)
 - apply/eq3_fun => s b s'.
   under eq2_exists do rewrite andC andA.
   rewrite ex2C.
@@ -155,7 +67,7 @@ Let assoc : BindLaws.associative bind.
 Proof.
 move=> A B C m f g; rewrite /bind /ret /hoare_bind /hoare_ret/=.
 case: m => prA poA/=; congr mk_hoare.
-- apply/funext => s; apply/propext; split.
+- apply/funext=> s; apply/propext; split.
   + move=> [[prAs poApre postpre]].
     split => // a s1 sas1; split=> [|b s2 s'bs2].
       exact: poApre.
@@ -164,7 +76,6 @@ case: m => prA poA/=; congr mk_hoare.
       by split=> // a s1 /poApre[].
     move=> b s1 [x [s2]] [] /poApre [fxs2] /[swap] s2bs1.
     exact.
-(* - exact: bindA. *)
 - apply: eq3_fun => s c s1.
   under eq2_exists do rewrite -ex_andl.
   rewrite ex3C; apply: eq_exists => a.
@@ -182,230 +93,69 @@ End hm.
 
 End Hoare.
 
-(** ** Monad *)
+HB.export Hoare.
 
-(** Easier to had future laws from there. *)
-(*
-HB.mixin Record isMonadHoare (S : Type) (ST : stateMonad S)
-    (M : Type -> Type) of Monad M := {
-      ht : forall (A: UU0) (m : M A), Prop ;
-      ht_bind (A B : UU0) (m : M A) (k : A -> M B) :
-        ht _ m -> (forall x, ht _ (k x)) -> ht _ (m >>= k) ;
+HB.about hoare.
 
-      wp: forall (A: UU0) (m : M A) (Q : A -> set S), set S ;
-
-      wp_ret : forall (A: UU0) (a : A) (Q : A -> set S), wp A (Ret a) Q = Q a;
-      wp_bind : forall (A B : UU0) (m : M A) (k : A -> M B) (Q : B -> set S),
-        wp _ (m >>= k) Q = wp _ m (fun x s=> wp _ (k x) Q s)
-    }.
+HB.mixin Record isMonadHoare
+(T : UU0) (N : monad)
+(ST : stateRunMonad T N)
+  (M : Type -> Type) of Monad M := {
+  valid_hoare : forall U : UU0, M U -> ST U -> Prop ;
+  valid_ret : forall (U : UU0) (x : U),
+    valid_hoare U (Ret x) (Ret x) ;
+  valid_bind : forall (U V : UU0) (h : M U) (m : ST U)
+      (h' : U -> M V) (k : U -> ST V),
+    valid_hoare U h m ->
+    (forall x, valid_hoare V (h' x) (k x)) ->
+    valid_hoare V (h >>= h') (m >>= k)
+}.
 
 #[short(type=hoareMonad)]
-HB.structure Definition MonadHoare (S : Type) (ST : stateMonad S) :=
-  {M of isMonadHoare S ST M &}. *)
+HB.structure Definition MonadHoare (T : UU0) (N : monad) (ST : stateRunMonad T N) :=
+  {M of isMonadHoare T N ST M & isMonad M & isFunctor M}.
 
-HB.export Hoare.
+Arguments valid_hoare {T N ST M U} _ _ : rename.
+
+Notation "{{ pre }} prog {{ post }}" :=
+  (valid_hoare (mk_hoare pre post) prog)
+  (at level 0,
+   format "'[' {{  pre  }} '/ ' prog '/ ' {{  post  }} ']'").
+
 From monae Require Import monad_model monad_transformer.
 
-Module TestM.
-Section st.
+Module HoareModel.
+Section vld_s.
+Context {T : UU0}.
+ (* {ST : stateRunMonad T }. *)
+Abbreviation HT := (hoare T).
+Abbreviation ST := (stateT T option_monad).
 
-Context {S : UU0}.
+Definition valid {U : UU0} (h : HT U) (m : ST U) : Prop :=
+  forall s, pre h s ->
+    (forall a s', runStateT m s = Ret (a, s') -> post h s a s').
 
-Let N : monad := option_monad.
-Definition M : stateMonad S := [the stateMonad S of stateT S N].
-(* Notation ms := (StateMonad.acto S). *)
+Lemma valid_ret : forall U (x : U), valid (hoare_ret x) (Ret x) .
+Proof. by move=> U u t /= P u' t'; rewrite runStateTret; case. Qed.
 
-HB.about stateRunMonad.
-Notation hs := (hoare S).
-
-(* Definition ht *)
-  (* (A : Type) (h: hs A) (m: M A) : Prop := valid_hoare h m. *)
-
-Definition wp (A : UU0) (h: hs A) (m: M A) (Q : A -> set S) : set S
- :=
-fun s=> match runStateT m s with
-| inr (a, s') => post h s a s' -> Q a s'
-| inl _ => True
-end.
-
-(* fun s=> match prog m s with *)
-(* | (a, s')=> Q a s' *)
-(* end. *)
-
-(* Lemma ht_bind (A B : UU0) (m : hs A) (k : A -> hs B) (p: M A) :
-  ht m -> (forall x, ht (k x)) -> ht (m >>= k).
+Lemma valid_bind : forall U V (h : HT U) (m : ST U)
+  (h' : U -> HT V) (k : U -> ST V),
+valid h m -> (forall x, valid (h' x) (k x)) -> valid (hoare_bind h h') (m >>= k).
 Proof.
-move=> Hm Hk s; move: Hm.
-case: m s=> /= pr pg po s + [Hpr Hpo]=> /(_ s Hpr) /=.
-rewrite state_bindE /comp /uncurry.
-case: (pg s) => a s' Hm.
-move: Hpo=> /(_ a s' Hm) Hpo.
-move: Hk=> /(_ a s' Hpo).
-case: (prog (k a)) => Hprk Hpg Hpok /=.
-by exists a, s'.
-Qed. *)
-
-(* Lemma wp_ret (A : UU0) (x : A) (Q : A -> S -> Prop) : *)
-  (* wp (Ret x) Q = Q x. *)
-(* Proof. done. Qed. *)
-(*  *)
-(* Lemma wp_bind (A B : UU0) (m : hs A) (k : A -> hs B) *)
-    (* (Q : B -> S -> Prop) : *)
-  (* wp (m >>= k) Q = wp m (fun x s => wp (k x) Q s). *)
-(* Proof. *)
-(* rewrite /wp; apply: funext=>s /=. *)
-(* rewrite state_bindE /comp /uncurry. *)
-(* by case : prog. *)
-(* Qed. *)
-(*  *)
-(* HB.about isMonadHoare.Build. *)
-(*  *)
-(* HB.instance Definition _ := isMonadHoare.Build S ms hs ht_bind wp_ret wp_bind. *)
-End st.
-End TestM.
-Export TestM.
-(* machinery to reason about WP / SP *)
-(* if I remember correctly, we need the consequence rules:
-- a weaken law and
-- a strengthen law *)
-(* Right now, all of this is commented because we try to extract this as laws or a record, for more modularity, *)
-(* Section hoare_state. *)
-(* Context {S : UU0} {M : stateMonad S}.
-Definition top : set S := fun s => True.
-Definition hget : hoare M S := {{top}} get {{ fun s x s' => s = s' /\ x = s}}.
-Definition hput (x : S) : hoare M unit := {{top}} put x {{fun _ _ f => f = x}}.
-End hoare_state.
-
-(* Section hoare_acto. *)
-Context {S : UU0}.
-Notation ms := (StateMonad.acto S).
-Notation hs := (hoare ms).
-
-
-Context {A : UU0}.
-Lemma consq {P P' : set S} (c : ms A ) {Q Q' : S -> A -> set S} :
-(forall i, P' i -> P i) -> (forall i x f , Q i x f -> Q' i x f ) ->
- ht ({{P}} c {{Q}}) -> ht ({{P'}} c {{Q'}}).
-Proof.
-move=> str wkn + s /= pr=> /(_ s) /=.
-move: str=>/(_ s pr) str /(_ str).
-by case: c; exact: wkn.
+move=> U V h m h' k valid_m valid_k s [Hpr Hpo] v t''.
+rewrite runStateTbind /=.
+case run_m: runStateT=> [[] | [u t]] //= H.
+(* have post_m : post h s u t := valid_m s Hpr u t run_m. *)
+exists u, t; split.
+- exact: valid_m.
+- apply: valid_k.
+  + by have := valid_m s Hpr u t run_m; exact: Hpo.
+  + exact: H.
 Qed.
 
-Lemma weaken {P : set S} (m : hs A) :
-ht m -> (forall s, P s -> pre m s) -> ht ({{ P }} prog m {{ post m }}).
-Proof.
-move=> Hm Hp.
-apply: consq.
-- exact: Hp.
-- move=> s a s'; exact.
-- exact: Hm.
-Qed.
+HB.about isMonadHoare.Build.
+HB.about hoare.
+HB.instance Definition _ := isMonadHoare.Build T option_monad ST HT valid_ret valid_bind.
 
-Lemma strengthen (m : hs A)
-(Q : S -> A -> S -> Prop) :
-ht m -> (forall s a s', post m s a s' -> Q s a s') -> ht ({{ pre m }} prog m {{ Q }}).
-Proof.
-move=> Hm Hp.
-apply: consq.
-- move=> s Hpr. exact: Hpr.
-- exact: Hp.
-- exact: Hm.
-Qed.
-
-Lemma wp_precondition (m : hs A) (Q : A -> S -> Prop) :
-ht ({{fun s=> wp m (post m s) s }} prog m {{ post m }}).
-Proof. done. Qed.
-
-Lemma wp_weakest (m : hs A) :
-ht m -> forall s, pre m s -> wp m (post m s) s .
-Proof. done. Qed.
-
-Lemma wp_get (Q : S -> S -> Prop) :
-  wp (hget) Q = (fun s => Q s s).
-Proof. done. Qed.
-
-Lemma wp_put (s' : S) (Q : unit -> S -> Prop) :
-  wp (hput s') Q = (fun _ => Q tt s').
-Proof. done. Qed.
-
-Definition incr : hoare (StateMonad.acto nat) nat := (hget >>= fun s=> hput (s + 1) >> hget). *)
-(* End hoare_acto. *)
-
-From FreerDPS Require Import effect freer contract.
-
-HB.mixin Record isContractSpecifier (S : Type) {Fx F : effect} `{F -<? Fx}
-    (M : Type -> Type) of MonadState S M := {
-      state_of_contract : forall (c : contract F S), Fx ~~> M ;
-      (* hoare_of_contract : forall (c : contract F S), Fx ~~> M *)
-    }.
-
-#[short(type=specMonad)]
-HB.structure Definition MonadSpec (S : Type) {Fx F : effect} `{Hf: F -<? Fx} :=
-  {M of isContractSpecifier S Fx F Hf M &}.
-
-  (* -------------------------------------------------------------------------- *)
-
-
-Module Tust.
-Section tmp.
-Context {S : UU0} {Fx F : effect} `{F -<? Fx}.
-Notation ms := (StateMonad.acto S).
-Notation hs := (hoare ms).
-
-(* This doesn't work right now because we need to create an A from nothing. *)
-Definition soc : forall (c : contract F S), Fx ~~> ms.
-move=> c A cmd s.
-apply: (_, _).
-- admit.
-- apply: gen_state_update.
-  + apply: H.
-  + apply: c.
-  + apply: s.
-  - apply: cmd.
-
-Check gen_state_update.
-Admitted.
-
-HB.instance Definition _ := isContractSpecifier.Build S Fx F H ms soc.
-End tmp.
-End Tust.
-Export Tust.
-(* -------------------------------------------------------------------------- *)
-(* -------------------------------------------------------------------------- *)
-(* -------------------------------------------------------------------------- *)
-(* -------------------------------------------------------------------------- *)
-(* -------------------------------------------------------------------------- *)
-HB.about stateMonad.
-Section tmp.
-Context {S : UU0}.
-(* Notation ms := (StateMonad.acto S). *)
-
-(* Definition hoare_of_contract {Fx F : effect} `{H: F -<? Fx} {MS : specMonad S H}  (c : contract F S) : Fx ~~> hoare MS
-  := fun U cmd =>
-  {{gen_requirement c ^~ cmd}}
-    state_of_contract c _ cmd
-  {{fun s u s' => s' = gen_state_update c s cmd u /\ gen_promise c s cmd u}}. *)
-
-Axiom state_update' : forall [F : effect] [T : UU0],
-contract F T -> T -> forall [U : UU0] {M : stateMonad T}, F U -> U -> M U.
-Definition gen_state_update' {S} (M : stateMonad S) {X : UU0} {Fx F : effect} `{F -<? Fx}
-    (c : contract F S)
-    (s : S) (cmd : Fx X) (x : X)
-  : M X :=
-  if prj cmd is Some cmd then state_update' c s cmd x else Ret x.
-Section hoare_freer.
-
-Check make_contract.
-
-
-Context {Fx F : effect} `{F -<? Fx} (T : Type) (c : contract F T).
-Context {M : stateMonad T}.
-Notation ms := (StateMonad.acto T).
-Notation hs := (hoare ms).
-Print store_update .
-
-Arguments gen_state_update' : simpl never.
-
-End hoare_freer.
-End tmp.
+End vld_s.
+End HoareModel.
